GCounter.thy: re-specify state-based CRDT

state-crdts/GCounter.thy
@@ -4,36 +4,40 @@ imports
   Network
 begin
 
-datatype ('id) operation = Increment 'id | Decrement 'id
-
 type_synonym ('id) state = "'id \<Rightarrow> int option"
+type_synonym ('id) operation = "'id state"
 
-fun update :: "'id state => 'id => (int => int) => ('id state) option" where
+fun option_max :: "int option \<Rightarrow> int option \<Rightarrow> int option"  where
+"option_max (Some x) (Some y) = Some (max x y)" |
+"option_max (Some x) None = Some x" | 
+"option_max None (Some y) = Some y" | 
+"option_max None None = None"
+
+fun update :: "'id state => 'id => (int => int) => ('id operation)" where
   "update x i fn = (case (x i) of
-      None       => Some(x(i := Some(fn 0)))
-    | Some (x_i) => Some(x(i := Some(fn x_i)))
-  )"
+      None       => x(i := Some(fn 0))
+    | Some (x_i) => x(i := Some(fn x_i)))"
+
+fun inc :: "'id \<Rightarrow> ('id state) \<Rightarrow> ('id operation)"  where
+"inc who st = update st who (\<lambda>x. x + 1)"
+
+fun dec :: "'id \<Rightarrow> ('id state) \<Rightarrow> ('id operation)"  where
+"dec who st = update st who (\<lambda>x. x - 1)"
 
 fun gcounter_op :: "('id operation) \<Rightarrow> ('id state) \<rightharpoonup> ('id state)" where
-  "gcounter_op (Increment i) x = update x i (\<lambda> y. y + 1)" |
-  "gcounter_op (Decrement i) x = update x i (\<lambda> y. y - 1)"
+"gcounter_op theirs ours = Some (\<lambda> x. option_max (theirs x) (ours x))"
 
 locale gcounter = network_with_ops _ gcounter_op "\<lambda> x. None"
 
 lemma (in gcounter) "gcounter_op x \<rhd> gcounter_op y = gcounter_op y \<rhd> gcounter_op x"
   sorry
-  (* by(case_tac x; case_tac y; auto simp add: kleisli_def) *)
 
 lemma (in gcounter) concurrent_operations_commute:
   assumes "xs prefix of i"
   shows "hb.concurrent_ops_commute (node_deliver_messages xs)"
   using assms
-  apply(clarsimp simp: hb.concurrent_ops_commute_def)
-  apply(unfold interp_msg_def, simp)
-  apply(case_tac "b"; case_tac "ba")
-   apply(auto simp add: kleisli_def)
   sorry
-
+  
 corollary (in gcounter) counter_convergence:
   assumes "set (node_deliver_messages xs) = set (node_deliver_messages ys)"
       and "xs prefix of i"
@@ -43,14 +47,14 @@ using assms by(auto simp add: apply_operations_def intro: hb.convergence_ext con
                 node_deliver_messages_distinct hb_consistent_prefix)
 
 context gcounter begin
-(* 
+
 sublocale sec: strong_eventual_consistency weak_hb hb interp_msg
   "\<lambda>ops. \<exists>xs i. xs prefix of i \<and> node_deliver_messages xs = ops" "\<lambda> x. None"
   apply(standard; clarsimp)
       apply(auto simp add: hb_consistent_prefix drop_last_message node_deliver_messages_distinct concurrent_operations_commute)
-   apply(metis (full_types) interp_msg_def counter_op.elims)
+   apply(metis (full_types) interp_msg_def gcounter_op.elims)
   using drop_last_message apply blast
-done
- *)
+  done
 end
+
 end
